wip

VST/progs64/verif_simple_allocator.v
@@ -1,3 +1,4 @@
+Require Import ZArith.
 Require Import VST.floyd.proofauto.
 Require Import VST.progs64.simple_allocator.
 #[export] Instance CompSpecs : compspecs. make_compspecs prog. Defined.
@@ -11,27 +12,114 @@ Check Vundef.
 Check reptype (Tstruct _slab noattr).
 Compute Ews.
 Definition tslab := Tstruct _slab noattr.
-Definition tfreelist := Tstruct _freelist noattr.
 Compute reptype tslab.
+
+Definition CHUNK_SIZE: Z := 1024.
+Definition ENTRY_SIZE: Z:= 4.
+Check memory_block.
+
 Definition slab_init_spec :=
   DECLARE _slab_init
-  WITH slab: val, p: val, chunksize: val, entry_size: val
-  PRE [ (tptr tslab), tptr tuchar, tulong, tulong ]
+  WITH slab: val, gv: globals, chunk: val
+  PRE [ (tptr tslab) ]
     PROP()
-    PARAMS (slab; p; chunksize; entry_size)
-    SEP (data_at Ews tslab (Vundef, (Vundef, (Vundef, Vundef))) slab)
+    PARAMS (slab) GLOBALS (gv)
+    SEP (data_at Ews tslab (Vundef, (Vundef, Vundef)) slab)
   POST [ tvoid ]
     PROP() RETURN()
-    SEP (data_at Ews tslab (chunksize, (entry_size, (p, Vnullptr))) slab).
+    SEP (data_at Ews tslab (Vptrofs (Ptrofs.repr CHUNK_SIZE), (Vptrofs (Ptrofs.repr ENTRY_SIZE), gv __space)) slab).
 
-Definition Gprog : funspecs := ltac:(with_library prog [slab_init_spec]).
-
+(*memory_block Ews CHUNK_SIZE p*)
 Check semax_body.
 Check⊤. 
+Check memory_block_data_at__tarray_tuchar_eq.
+Check tptr tuchar.
+(*Definition slab_inv (slab: val) (p: val) (buf: val) :=*)
+  (*field_at slab (DOT _chunk) *)
+Print memory_block.
+Print valid_pointer'.
+Check memory_block_valid_pointer.
+Check Vptr.
+
+Print gfield.
+Search "array".
+Definition slab_alloc_spec :=
+  DECLARE _slab_alloc
+  WITH slab: val, chunksize: Z, entry_size: Z, chunk: val, chunk_block: block, 
+  b: block, gv: globals
+  PRE [ tptr tslab ]
+    PROP(entry_size <= chunksize;
+        0 <= chunksize <= Ptrofs.max_unsigned;
+        0 <= entry_size <= Ptrofs.max_unsigned;
+        slab <> nullval;
+        chunk = Vptr chunk_block (Ptrofs.repr 0);
+        chunk_block = b
+    )
+    PARAMS (slab)
+    GLOBALS (gv)
+    SEP (
+        memory_block Ews CHUNK_SIZE (Vptr b (Ptrofs.repr 0));
+        data_at Ews tslab (Vptrofs (Ptrofs.repr chunksize),
+          (Vptrofs (Ptrofs.repr entry_size),
+            chunk)) slab
+    )
+  POST [ tptr tvoid ] ∃res:val, 
+    PROP()
+    (*LOCAL(lvar _r chunk)*)
+    RETURN(chunk)
+    SEP (valid_pointer chunk;
+        data_at Ews tslab (Vptrofs (Ptrofs.repr (chunksize - entry_size)),
+        (Vptrofs (Ptrofs.repr entry_size),
+            offset_val entry_size chunk)) slab
+    ).
+
+Definition Gprog : funspecs := ltac:(with_library prog [slab_alloc_spec; slab_init_spec]).
+
 Lemma body_slab_init: semax_body Vprog Gprog f_slab_init slab_init_spec.
 Proof.
   start_function.
   repeat forward.
   entailer!.
 Qed.
+
+
+Check Vprog.
+(* seems important ingrediant *)
+Check memory_block_valid_pointer.
+Print memory_block.
+Check memory_block_data_at__tarray_tuchar_eq.
+(*Check fun (gv: globals) => memory_block_data_at__tarray_tuchar_eq Ews (gv __space) CHUNK_SIZE.*)
+(*Check fun (gv: globals) => memory_block_valid_pointer Ews CHUNK_SIZE (gv __space).*)
+(*Search memory_block .*)
+(*Check Ptrofs.unsigned_repr.*)
+
+    (*field_at Ews tslab (DOT Check_entry_size) (Vlong (Int64.repr entry_size)) slab;*)
+    (*field_at Ews tslab (DOT _chunksize) (Vlong (Int64.repr chunksize)) slab*)
+
+(*Search "addrof".*)
+Print  offset_val.
+
+(* valid_pointer chunk must be provable from this *)
+(*Definition slab_invariant (slab: val) chunksize entry_size chunk chunk_block chunk_ofs (gv: globals)  :=*)
+  (*data_at Ews tslab (Vptrofs (Ptrofs.repr chunksize), (Vptrofs (Ptrofs.repr entry_size), chunk)) slab*)
+ (*∗  data_at Ews (tptr tuchar) (Vptr chunk_block chunk_ofs) chunk.*)
+(*Check slab_invariant.*)
+(*Search is_pointer_or_null.*)
+
+Lemma body_slab_alloc: semax_body Vprog Gprog f_slab_alloc slab_alloc_spec.
+Proof.
+  start_function.
+  repeat forward.
+  forward_if.
+  (*Search Int.unsigned (Int.repr _).*)
+  (*Check Z.nle_gt.*)
+  - forward. lia.
+  - repeat forward.
+    Check memory_block_valid_pointer.
+    + rewrite (memory_block_valid_pointer Ews CHUNK_SIZE (Vptr b (Ptrofs.repr 0)) 0).
+      rewrite offset_val_zero_Vptr. entailer. 
+      * split;auto. lia.
+      * auto.
+Qed.
+
 End mpred.
